Verified egress parser.

examples/sampler/common.v
@@ -35,8 +35,213 @@ Definition ge := ltac:(get_ge am_ge prog).
 
 Definition header_sample_t: P4Type := ltac:(get_type "header_sample_t" ge).
 Definition metadata_t: P4Type := ltac:(get_type "metadata_t" ge).
+Definition bridge_t: P4Type := ltac:(get_type "bridge_t" ge).
+Definition sample_t: P4Type := ltac:(get_type "sample_t" ge).
 Definition tcp_h: P4Type := ltac:(get_type "tcp_h" ge).
 Definition udp_h: P4Type := ltac:(get_type "udp_h" ge).
 Definition ipv4_h: P4Type := ltac:(get_type "ipv4_h" ge).
 Definition ethernet_h: P4Type := ltac:(get_type "ethernet_h" ge).
 Definition MeterColor_t: P4Type := ltac:(get_type "MeterColor_t" ge).
+
+Definition IP_PROTOCOLS_TCP: Z := 6.
+Definition IP_PROTOCOLS_UDP: Z := 17.
+
+Record ipv4_rec := {
+    ipv4_version: Val;
+    ipv4_ihl: Val;
+    ipv4_diffserv: Val;
+    ipv4_total_len: Val;
+    ipv4_identification: Val;
+    ipv4_flags: Val;
+    ipv4_frag_offset: Val;
+    ipv4_ttl: Val;
+    ipv4_protocol: Val;
+    ipv4_hdr_checksum: Val;
+    ipv4_src_addr: Val;
+    ipv4_dst_addr: Val;
+  }.
+
+Definition ipv4_repr_val (ipv4: ipv4_rec): Val :=
+  ValBaseHeader
+    [("version", ipv4_version ipv4);
+     ("ihl", ipv4_ihl ipv4);
+     ("diffserv", ipv4_diffserv ipv4);
+     ("total_len", ipv4_total_len ipv4);
+     ("identification", ipv4_identification ipv4);
+     ("flags", ipv4_flags ipv4);
+     ("frag_offset", ipv4_frag_offset ipv4);
+     ("ttl", ipv4_ttl ipv4);
+     ("protocol", ipv4_protocol ipv4);
+     ("hdr_checksum", ipv4_hdr_checksum ipv4);
+     ("src_addr", ipv4_src_addr ipv4);
+     ("dst_addr", ipv4_dst_addr ipv4)] true.
+
+Definition is_tcp ipv4: bool :=
+  Val_eqb (ipv4_protocol ipv4) (P4BitV 8 IP_PROTOCOLS_TCP).
+
+Definition is_udp ipv4: bool :=
+  Val_eqb (ipv4_protocol ipv4) (P4BitV 8 IP_PROTOCOLS_UDP).
+
+Definition protocol_extract_result
+  (ipv4: ipv4_rec) (result: Val) (header: Sval): Sval :=
+  if is_tcp ipv4 then update "tcp" (eval_val_to_sval result) header
+  else if is_udp ipv4 then update "udp" (eval_val_to_sval result) header
+       else header.
+
+Record header_sample_rec := {
+    header_sample_bridge: Sval;
+    header_sample_sample: Sval;
+    header_sample_ethernet: Sval;
+    header_sample_ipv4: Sval;
+    header_sample_tcp: Sval;
+    header_sample_udp: Sval;
+  }.
+
+Definition hdr (hsample: header_sample_rec) :=
+  ValBaseStruct
+    [("bridge", header_sample_bridge hsample);
+     ("sample", header_sample_sample hsample);
+     ("ethernet", header_sample_ethernet hsample);
+     ("ipv4", header_sample_ipv4 hsample);
+     ("tcp", header_sample_tcp hsample);
+     ("udp", header_sample_udp hsample)].
+
+Lemma force_cast_P4BitV_eq: forall w v,
+    force ValBaseNull (@Ops.eval_cast Info (TypBit w) (P4BitV w v)) = P4BitV w v.
+Proof.
+  intros. unfold P4BitV. simpl. f_equal. rewrite P4Arith.bit_to_lbool_back.
+  unfold P4Arith.BitArith.mod_bound. rewrite Zmod_mod.
+  change (v mod _) with (P4Arith.BitArith.mod_bound w v).
+  rewrite P4Arith.to_lbool_bit_mod. reflexivity.
+Qed.
+
+Lemma abs_ipv4_hdr_eq_eq: forall ipv4 hsample w v,
+    abs_eq
+      (get "protocol"
+         (get "ipv4"
+            (update "ipv4" (eval_val_to_sval (ipv4_repr_val ipv4))
+               (hdr hsample))))
+      (build_abs_unary_op (@Ops.eval_cast Info (TypBit w))
+         (eval_val_to_sval (P4BitV w v))) =
+      eval_val_to_sval
+        (force ValBaseNull
+           (Ops.eval_binary_op Eq (ipv4_protocol ipv4) (P4BitV w v))).
+Proof.
+  intros. rewrite get_update_same; auto.
+  unfold build_abs_unary_op. rewrite eval_sval_to_val_eq.
+  rewrite force_cast_P4BitV_eq. unfold ipv4_repr_val. simpl get. unfold abs_eq.
+  unfold build_abs_binary_op. rewrite !eval_sval_to_val_eq. reflexivity.
+Qed.
+
+Lemma is_sval_true_binary_op_eq: forall v1 v2,
+  is_sval_true
+    (eval_val_to_sval (force ValBaseNull (Ops.eval_binary_op Eq v1 v2))) ->
+  Val_eqb v1 v2 = true.
+Proof.
+  intros. unfold Ops.eval_binary_op in H.
+  remember (Ops.eval_binary_op_eq _ _).
+  destruct o eqn:?H; simpl in H; [destruct b|]; [|exfalso; auto..].
+  symmetry in Heqo. apply Ops.eval_binary_op_eq_eq in Heqo.
+  rewrite <- Val_eqb_eq_iff in Heqo. assumption.
+Qed.
+
+Lemma is_sval_false_binary_op_eq: forall v1 v2,
+  is_sval_false
+    (eval_val_to_sval (force ValBaseNull (Ops.eval_binary_op Eq v1 v2))) ->
+  Val_eqb v1 v2 = false.
+Proof.
+  intros. unfold Ops.eval_binary_op in H.
+  remember (Ops.eval_binary_op_eq _ _).
+  destruct o eqn:?H; simpl in H; [destruct b|]. 1, 3: exfalso; assumption.
+  symmetry in Heqo. apply Ops.eval_binary_op_neq_neq in Heqo.
+  rewrite <- Val_eqb_eq_iff in Heqo. apply Bool.not_true_is_false in Heqo.
+  assumption.
+Qed.
+
+Record ethernet_rec := {
+    ethernet_dst_addr: Val;
+    ethernet_src_addr: Val;
+    ethernet_ether_type: Val;
+  }.
+
+Definition ethernet_repr_val (ether: ethernet_rec) : Val :=
+  ValBaseHeader
+    [("dst_addr", ethernet_dst_addr ether);
+     ("src_addr", ethernet_src_addr ether);
+     ("ether_type", ethernet_ether_type ether)] true.
+
+Definition ethernet_extract_result
+  (header: Sval) (ether: ethernet_rec) (ipv4: ipv4_rec)
+  (result: Val): Sval :=
+  protocol_extract_result ipv4 result
+    (update "ipv4" (eval_val_to_sval (ipv4_repr_val ipv4))
+       (update "ethernet" (eval_val_to_sval (ethernet_repr_val ether))
+          header)).
+
+Definition ETHERTYPE_IPV4: Z := 0x800.
+
+Lemma abs_ether_eq_eq: forall ether hsample w v,
+    abs_eq
+      (get "ether_type"
+         (get "ethernet"
+            (update "ethernet" (eval_val_to_sval (ethernet_repr_val ether))
+               (hdr hsample))))
+      (build_abs_unary_op (@Ops.eval_cast Info (TypBit w))
+         (eval_val_to_sval (P4BitV w v))) =
+      eval_val_to_sval
+        (force ValBaseNull
+           (Ops.eval_binary_op Eq (ethernet_ether_type ether) (P4BitV w v))).
+Proof.
+  intros. rewrite get_update_same; auto.
+  unfold build_abs_unary_op. rewrite eval_sval_to_val_eq.
+  rewrite force_cast_P4BitV_eq. unfold ethernet_repr_val. simpl get. unfold abs_eq.
+  unfold build_abs_binary_op. rewrite !eval_sval_to_val_eq. reflexivity.
+Qed.
+
+Definition hdr_init: header_sample_rec :=
+  Build_header_sample_rec
+    (ValBaseHeader
+       [("contains_sample", P4Bit_ 8)] (Some false))
+    (ValBaseHeader
+       [("dmac", P4Bit_ 48);
+        ("smac", P4Bit_ 48);
+        ("etype", P4Bit_ 16);
+        ("srcip", P4Bit_ 32);
+        ("dstip", P4Bit_ 32);
+        ("num_pkts", P4Bit_ 32)] (Some false))
+    (ValBaseHeader
+       [("dst_addr", P4Bit_ 48);
+        ("src_addr", P4Bit_ 48);
+        ("ether_type", P4Bit_ 16)] (Some false))
+    (ValBaseHeader
+       [("version", P4Bit_ 4);
+        ("ihl", P4Bit_ 4);
+        ("diffserv", P4Bit_ 8);
+        ("total_len", P4Bit_ 16);
+        ("identification", P4Bit_ 16);
+        ("flags", P4Bit_ 3);
+        ("frag_offset", P4Bit_ 13);
+        ("ttl", P4Bit_ 8);
+        ("protocol", P4Bit_ 8);
+        ("hdr_checksum", P4Bit_ 16);
+        ("src_addr", P4Bit_ 32);
+        ("dst_addr", P4Bit_ 32)]
+       (Some false))
+    (ValBaseHeader
+       [("src_port", P4Bit_ 16);
+        ("dst_port", P4Bit_ 16);
+        ("seq_no", P4Bit_ 32);
+        ("ack_no", P4Bit_ 32);
+        ("data_offset", P4Bit_ 4);
+        ("res", P4Bit_ 4);
+        ("flags", P4Bit_ 8);
+        ("window", P4Bit_ 16);
+        ("checksum", P4Bit_ 16);
+        ("urgent_ptr", P4Bit_ 16)]
+       (Some false))
+    (ValBaseHeader
+        [("src_port", P4Bit_ 16);
+         ("dst_port", P4Bit_ 16);
+         ("hdr_length", P4Bit_ 16);
+         ("checksum", P4Bit_ 16)]
+        (Some false)).
